Rename lft_tok to lft_alive and lft_eter to lft_etern

nola/iris/lft.v
@@ -80,12 +80,12 @@ Proof. by move=> ? /lft_eqtop_meet_r. Qed.
 
 (** ** Lifetime tokens *)
 
-(** Atomic lifetime token *)
-Local Definition alft_tok `{!lftG Σ} (a : alft) (q : Qp) : iProp Σ :=
+(** Atomic alive lifetime token *)
+Local Definition alft_alive `{!lftG Σ} (a : alft) (q : Qp) : iProp Σ :=
   own a (Cinl (DfracOwn q)).
-(** Lifetime token *)
-Notation lft_tok α q := ([∗ mset] a ∈ α, alft_tok a q)%I.
-Notation "q .[ α ]" := (lft_tok α q)
+(** Alive lifetime token *)
+Notation lft_alive α q := ([∗ mset] a ∈ α, alft_alive a q)%I.
+Notation "q .[ α ]" := (lft_alive α q)
   (format "q .[ α ]", at level 2, left associativity) : bi_scope.
 
 (** Dead atomic lifetime token *)
@@ -100,11 +100,11 @@ Proof. exact: seal_eq. Qed.
 Notation "[† α ]" := (lft_dead α) (format "[† α ]") : bi_scope.
 
 (** Eternal atomic lifetime token *)
-Local Definition alft_eter `{!lftG Σ} (a : alft) : iProp Σ :=
+Local Definition alft_etern `{!lftG Σ} (a : alft) : iProp Σ :=
   own a (Cinl DfracDiscarded).
 (** Eternal lifetime token *)
-Notation lft_eter α := ([∗ mset] a ∈ α, alft_eter a)%I.
-Notation "[∞ α ]" := (lft_eter α) (format "[∞ α ]") : bi_scope.
+Notation lft_etern α := ([∗ mset] a ∈ α, alft_etern a)%I.
+Notation "[∞ α ]" := (lft_etern α) (format "[∞ α ]") : bi_scope.
 
 Section lft.
   Context `{!lftG Σ}.
@@ -112,56 +112,56 @@ Section lft.
   (** Dead and eternal lifetime tokens are persistent *)
   #[export] Instance lft_dead_persistent {α} : Persistent [†α].
   Proof. rewrite lft_dead_unseal. exact _. Qed.
-  Fact lft_eter_persistent {α} : Persistent [∞α].
+  Fact lft_etern_persistent {α} : Persistent [∞α].
   Proof. exact _. Qed.
 
-  (** Lifetime, dead, eternal lifetime tokens are timeless *)
-  Fact lft_tok_timeless {α q} : Timeless q.[α].
+  (** Alive, dead, eternal lifetime tokens are timeless *)
+  Fact lft_alive_timeless {α q} : Timeless q.[α].
   Proof. exact _. Qed.
   #[export] Instance lft_dead_timeless {α} : Timeless [†α].
   Proof. rewrite lft_dead_unseal. exact _. Qed.
-  Fact lft_eter_timeless {α} : Timeless [∞α].
+  Fact lft_etern_timeless {α} : Timeless [∞α].
   Proof. exact _. Qed.
 
-  (** Lifetime and dead lifetime tokens can't coexist *)
-  Lemma lft_tok_dead {α q} : q.[α] -∗ [†α] -∗ False.
+  (** Alive and dead lifetime tokens can't coexist *)
+  Lemma lft_alive_dead {α q} : q.[α] -∗ [†α] -∗ False.
   Proof.
     rewrite lft_dead_unseal. iIntros "q". iDestruct 1 as (a) "[%e †]".
     rewrite big_sepMS_elem_of; [|done].
     by iDestruct (own_valid_2 with "q †") as "%".
   Qed.
   (** Eternal and dead lifetime tokens can't coexist *)
-  Lemma lft_eter_dead {α} : [∞α] -∗ [†α] -∗ False.
+  Lemma lft_etern_dead {α} : [∞α] -∗ [†α] -∗ False.
   Proof.
     rewrite lft_dead_unseal. iIntros "∞". iDestruct 1 as (a) "[%e †]".
     rewrite big_sepMS_elem_of; [|done].
     by iDestruct (own_valid_2 with "∞ †") as "%".
   Qed.
-  (** The fraction of a lifetime token is no more than [1] *)
-  Lemma lft_tok_valid {α q} : α ≠ ⊤ → q.[α] -∗ ⌜q ≤ 1⌝%Qp.
+  (** The fraction of an alive lifetime token is no more than [1] *)
+  Lemma lft_alive_valid {α q} : α ≠ ⊤ → q.[α] -∗ ⌜q ≤ 1⌝%Qp.
   Proof.
     case: (gmultiset_choose_or_empty α); [|done]=> [[a ?]_]. iIntros "α".
     iDestruct (big_sepMS_elem_of with "α") as "a"; [done|].
     by iDestruct (own_valid with "a") as %?.
   Qed.
 
-  (** Lifetime token is fractional *)
-  Local Instance alft_tok_fract {a} : Fractional (alft_tok a)%I.
+  (** Alive lifetime token is fractional *)
+  Local Instance alft_alive_fract {a} : Fractional (alft_alive a)%I.
   Proof. move=> ??. by rewrite -own_op -Cinl_op. Qed.
-  Local Instance alft_tok_as_fract {a q} :
-    AsFractional (alft_tok a q) (alft_tok a) q.
+  Local Instance alft_alive_as_fract {a q} :
+    AsFractional (alft_alive a q) (alft_alive a) q.
   Proof. split; [done|exact _]. Qed.
-  #[export] Instance lft_tok_fract {α} : Fractional (λ q, q.[α])%I.
+  #[export] Instance lft_alive_fract {α} : Fractional (λ q, q.[α])%I.
   Proof. exact _. Qed.
-  #[export] Instance lft_tok_as_fract {α q} :
+  #[export] Instance lft_alive_as_fract {α q} :
     AsFractional q.[α] (λ q, q.[α])%I q.
   Proof. split; [done|exact _]. Qed.
-  #[export] Instance lft_tok_fract_frame {p α} `{!FrameFractionalQp q r s} :
+  #[export] Instance lft_alive_fract_frame {p α} `{!FrameFractionalQp q r s} :
     Frame p q.[α] r.[α] s.[α] | 5.
   Proof. apply: frame_fractional. Qed.
 
-  (** Combine lifetime tokens *)
-  Lemma lft_tok_combine {α β q r} :
+  (** Combine alive lifetime tokens *)
+  Lemma lft_alive_combine {α β q r} :
     q.[α] -∗ r.[β] -∗ ∃ s, s.[α ⊓ β] ∗ (s.[α ⊓ β] -∗ q.[α] ∗ r.[β]).
   Proof.
     case: (Qp.lower_bound q r)=> [s[t[t'[->->]]]]. iIntros "[α α'][β β']".
@@ -186,7 +186,7 @@ Section lft.
   Qed.
 
   (** Eternalize a lifetime *)
-  Local Lemma alft_eternalize {a q} : alft_tok a q ==∗ alft_eter a.
+  Local Lemma alft_eternalize {a q} : alft_alive a q ==∗ alft_etern a.
   Proof.
     iIntros "a". iApply (own_update with "a").
     apply csum_update_l, dfrac_discard_update.
@@ -197,8 +197,8 @@ Section lft.
     iApply alft_eternalize.
   Qed.
 
-  (** Get a lifetime token out of an eternal lifetime token *)
-  Local Lemma alft_eter_tok {a} : alft_eter a ==∗ ∃ q, alft_tok a q.
+  (** Get an alive lifetime token out of an eternal lifetime token *)
+  Local Lemma alft_etern_alive {a} : alft_etern a ==∗ ∃ q, alft_alive a q.
   Proof.
     iIntros "∞".
     iMod (own_updateP (λ a, ∃ q, a = Cinl (DfracOwn q)) with "∞") as
@@ -206,23 +206,23 @@ Section lft.
     eapply csum_updateP_l; [exact dfrac_restore_update|]=>/= ?[?->].
     by eexists _.
   Qed.
-  Local Lemma alftl_eter_tok {al} :
-    ([∗ list] a ∈ al, alft_eter a) ==∗ ∃ q, [∗ list] a ∈ al, alft_tok a q.
+  Local Lemma alftl_etern_alive {al} :
+    ([∗ list] a ∈ al, alft_etern a) ==∗ ∃ q, [∗ list] a ∈ al, alft_alive a q.
   Proof.
     elim: al=> [|a al IH]/=; [iIntros "_"; by iExists 1%Qp|].
-    iIntros "[∞ al]". iMod (alft_eter_tok with "∞") as (q) "a".
+    iIntros "[∞ al]". iMod (alft_etern_alive with "∞") as (q) "a".
     iMod (IH with "al") as (r) "al". iModIntro.
     case: (Qp.lower_bound q r)=> [s[t[t'[->->]]]].
     iExists s. iDestruct "a" as "[$ _]". iStopProof. do 3 f_equiv.
     iDestruct 1 as "[$ ?]".
   Qed.
-  Lemma lft_eter_tok {α} : [∞α] ==∗ ∃ q, q.[α].
-  Proof. setoid_rewrite big_opMS_elements. apply alftl_eter_tok. Qed.
+  Lemma lft_etern_alive {α} : [∞α] ==∗ ∃ q, q.[α].
+  Proof. setoid_rewrite big_opMS_elements. apply alftl_etern_alive. Qed.
 
-  (** Lifetime token over [⊤]/[⊓] *)
-  Lemma lft_tok_top {q} : ⊢ q.[⊤].
+  (** Alive lifetime token over [⊤]/[⊓] *)
+  Lemma lft_alive_top {q} : ⊢ q.[⊤].
   Proof. by apply big_sepMS_empty'. Qed.
-  Lemma lft_tok_meet {α β q} : q.[α ⊓ β] ⊣⊢ q.[α] ∗ q.[β].
+  Lemma lft_alive_meet {α β q} : q.[α ⊓ β] ⊣⊢ q.[α] ∗ q.[β].
   Proof. by apply big_sepMS_disj_union. Qed.
 
   (** Dead lifetime token over [⊤]/[⊓] *)
@@ -242,15 +242,15 @@ Section lft.
   Proof. iIntros. rewrite lft_dead_meet. by iRight. Qed.
 
   (** Eternal lifetime token over [⊤]/[⊓] *)
-  Lemma lft_eter_top : ⊢ [∞⊤].
+  Lemma lft_etern_top : ⊢ [∞⊤].
   Proof. by apply big_sepMS_empty'. Qed.
-  Lemma lft_eter_meet {α β} : [∞α ⊓ β] ⊣⊢ [∞α] ∗ [∞β].
+  Lemma lft_etern_meet {α β} : [∞α ⊓ β] ⊣⊢ [∞α] ∗ [∞β].
   Proof. by apply big_sepMS_disj_union. Qed.
 
-  (** Access a lifetime token using [⊑] *)
-  Local Lemma alftl_incl_tok_acc {α q} bl : bl ⊆ elements α →
-    q.[α] ⊢ ∃ r, ([∗ list] b ∈ bl, alft_tok b r) ∗
-      (([∗ list] b ∈ bl, alft_tok b r) -∗ q.[α]).
+  (** Access an alive lifetime token using [⊑] *)
+  Local Lemma alftl_incl_alive_acc {α q} bl : bl ⊆ elements α →
+    q.[α] ⊢ ∃ r, ([∗ list] b ∈ bl, alft_alive b r) ∗
+      (([∗ list] b ∈ bl, alft_alive b r) -∗ q.[α]).
   Proof.
     elim: bl q=> /=[|b bl IH] q inc.
     { iIntros. iExists 1%Qp. iSplit; [done|]. by iFrame. }
@@ -258,17 +258,17 @@ Section lft.
     iDestruct (big_sepMS_elem_of_acc _ _ b with "α") as "[b →α]".
     { rewrite -gmultiset_elem_of_elements. set_solver. }
     case: (Qp.lower_bound r (q/2)%Qp)=> [s[t[t'[->eq]]]].
-    have -> : alft_tok b (q / 2) ⊣⊢ alft_tok b s ∗ alft_tok b t'.
+    have -> : alft_alive b (q / 2) ⊣⊢ alft_alive b s ∗ alft_alive b t'.
     { by rewrite eq fractional. }
     iExists _. iDestruct "b" as "[$ b']". setoid_rewrite fractional.
     rewrite big_sepL_sep. iDestruct "bl" as "[$ bl']". iIntros "[b bl]".
     iDestruct ("→α" with "[$b $b']") as "$". iApply "→α'". iFrame.
   Qed.
-  Lemma lft_incl_tok_acc {α β q} :
+  Lemma lft_incl_alive_acc {α β q} :
     α ⊑ β → q.[α] ⊢ ∃ r, r.[β] ∗ (r.[β] -∗ q.[α]).
   Proof.
     move=> βα. iIntros "α".
-    iDestruct (alftl_incl_tok_acc (elements β) with "α") as (r) "[bl →α]";
+    iDestruct (alftl_incl_alive_acc (elements β) with "α") as (r) "[bl →α]";
       [done|]. iExists _. rewrite -big_opMS_elements. iFrame.
   Qed.
 
@@ -285,15 +285,15 @@ Section lft.
   Proof. solve_proper. Qed.
 
   (** Modify an eternal lifetime token using [⊑] *)
-  Lemma lft_incl_eter {α β} : α ⊑ β → [∞α] ⊢ [∞β].
+  Lemma lft_incl_etern {α β} : α ⊑ β → [∞α] ⊢ [∞β].
   Proof.
     rewrite !big_opMS_elements=> αβ. iIntros "α". iApply big_sepL_forall.
     iIntros (?? eq). apply elem_of_list_lookup_2 in eq.
     rewrite big_sepL_elem_of; [done|]. by apply αβ.
   Qed.
-  #[export] Instance lft_eter_mono : Proper ((⊑) ==> (⊢)) (λ α, [∞α])%I.
-  Proof. move=> >. exact lft_incl_eter. Qed.
-  #[export] Instance lft_eter_mono' :
+  #[export] Instance lft_etern_mono : Proper ((⊑) ==> (⊢)) (λ α, [∞α])%I.
+  Proof. move=> >. exact lft_incl_etern. Qed.
+  #[export] Instance lft_etern_mono' :
     Proper (flip (⊑) ==> flip (⊢)) (λ α, [∞α])%I.
   Proof. solve_proper. Qed.
 End lft.
@@ -320,16 +320,16 @@ Section lft.
   #[export] Instance lft_sincl_timeless {α β} : Timeless (α ⊑□ β).
   Proof. rewrite lft_sincl_unseal. exact _. Qed.
 
-  (** Access a lifetime token by [⊑□] *)
-  Lemma lft_sincl_tok_acc {α β q} :
+  (** Access an alive lifetime token by [⊑□] *)
+  Lemma lft_sincl_alive_acc {α β q} :
     α ⊑□ β -∗ q.[α] ==∗ ∃ r, r.[β] ∗ (r.[β] -∗ q.[α]).
   Proof.
     rewrite lft_sincl_unseal. iIntros "[†|[%[% γ]]] α".
-    { iDestruct (lft_tok_dead with "α †") as "[]". }
-    iMod (lft_eter_tok with "γ") as (r) "γ". iModIntro.
-    iDestruct (lft_tok_combine with "α γ") as (s) "[αγ →]".
-    iDestruct (lft_incl_tok_acc with "αγ") as (?) "[β →α]"; [done|]. iExists _.
-    iFrame "β". iIntros "β". iDestruct ("→α" with "β") as "αγ".
+    { iDestruct (lft_alive_dead with "α †") as "[]". }
+    iMod (lft_etern_alive with "γ") as (r) "γ". iModIntro.
+    iDestruct (lft_alive_combine with "α γ") as (s) "[αγ →]".
+    iDestruct (lft_incl_alive_acc with "αγ") as (?) "[β →α]"; [done|].
+    iExists _. iFrame "β". iIntros "β". iDestruct ("→α" with "β") as "αγ".
     iDestruct ("→" with "αγ") as "[$ _]".
   Qed.
 
@@ -338,22 +338,22 @@ Section lft.
   Proof.
     rewrite lft_sincl_unseal. iIntros "[$|[%[% γ]]] †"; [done|].
     rewrite lft_incl_dead; [|done]. rewrite lft_dead_meet.
-    iDestruct "†" as "[$|†]". iDestruct (lft_eter_dead with "γ †") as "[]".
+    iDestruct "†" as "[$|†]". iDestruct (lft_etern_dead with "γ †") as "[]".
   Qed.
 
   (** Modify an eternal lifetime token using [⊑□] *)
-  Lemma lft_sincl_eter {α β} : α ⊑□ β ⊢ [∞α] -∗ [∞β].
+  Lemma lft_sincl_etern {α β} : α ⊑□ β ⊢ [∞α] -∗ [∞β].
   Proof.
     rewrite lft_sincl_unseal. iIntros "[†|[%γ[%inc γ]]] α".
-    { iDestruct (lft_eter_dead with "α †") as "[]". }
-    iApply lft_incl_eter; [done|]. by iSplit.
+    { iDestruct (lft_etern_dead with "α †") as "[]". }
+    iApply lft_incl_etern; [done|]. by iSplit.
   Qed.
 
   (** [⊑] entails [⊑□] *)
   Lemma lft_incl_sincl {α β} : α ⊑ β → ⊢ α ⊑□ β.
   Proof.
     rewrite lft_sincl_unseal=> ?. iRight. iExists ⊤.
-    iSplit; [|by iApply lft_eter_top]. iPureIntro. by rewrite right_id.
+    iSplit; [|by iApply lft_etern_top]. iPureIntro. by rewrite right_id.
   Qed.
 
   (** [⊑□] is reflexive, is transitive, has the maximum [⊤] *)
@@ -364,7 +364,7 @@ Section lft.
     rewrite lft_sincl_unseal. iIntros "[$|[%δ[% δ]]]"; [by iIntros|].
     iIntros "[†|[%δ'[% δ']]]".
     { iLeft. rewrite lft_incl_dead; [|done]. rewrite lft_dead_meet.
-      iDestruct "†" as "[$|†]". iDestruct (lft_eter_dead with "δ †") as "[]". }
+      iDestruct "†" as "[$|†]". iDestruct (lft_etern_dead with "δ †") as "[]". }
     iRight. iExists (δ ⊓ δ'). iFrame "δ δ'". iPureIntro. etrans; [|done].
     rewrite assoc. by apply lft_incl_meet_mono_l.
   Qed.
@@ -376,13 +376,13 @@ Section lft.
   Proof. rewrite lft_sincl_unseal. by iIntros "$". Qed.
 
   (** An eternal lifetime is the maximum w.r.t. [⊑□] *)
-  Lemma lft_sincl_by_eter {α} : [∞α] ⊢ ∀ β, β ⊑□ α.
+  Lemma lft_sincl_by_etern {α} : [∞α] ⊢ ∀ β, β ⊑□ α.
   Proof.
     rewrite lft_sincl_unseal. iIntros "#∞ %β". iRight. iExists _. iFrame "∞".
     iPureIntro. exact lft_incl_meet_r.
   Qed.
   Lemma lft_eternalize_sincl {α q} : q.[α] ==∗ ∀ β, β ⊑□ α.
-  Proof. rewrite -lft_sincl_by_eter. apply lft_eternalize. Qed.
+  Proof. rewrite -lft_sincl_by_etern. apply lft_eternalize. Qed.
 
   (** [⊓] is the lub w.r.t. [⊑□] *)
   Lemma lft_sincl_meet_l {α β} : ⊢ α ⊓ β ⊑□ α.
